rustfrontend/RustIRown.v
@@ -196,10 +196,26 @@ Definition own_check_assign (own: own_env) (p: place) : option own_env :=
 (* Drop place state *)
 
 Inductive drop_place_state : Type :=
-| drop_fully_owned
+| drop_fully_owned_comp
+    (* drop the composite and then drop the box *)
+    (p: place) (l: list place) : drop_place_state
+| drop_fully_owned_box
     (l: list place) : drop_place_state
 .
-  
+
+Definition gen_drop_place_state (p: place) : drop_place_state :=
+  match split_fully_own_place p (typeof_place p) with
+  | nil => drop_fully_owned_box nil
+  | p' :: l =>
+      match typeof_place p' with
+      | Tstruct _ _
+      | Tvariant _ _ =>
+          drop_fully_owned_comp p' l
+      | _ =>
+          drop_fully_owned_box (p' :: l)
+      end
+  end.
+          
 (** Continuation *)
   
 Inductive cont : Type :=
@@ -393,13 +409,13 @@ Inductive step_dropplace : state -> trace -> state -> Prop :=
 | step_dropplace_init1: forall f p ps k le own m full
     (* p is not owned, so just skip it (How to relate this case with
     RustIRsem because drop elaboration removes this place earlier in
-    generate_drop_flag *)
+    generate_drop_flag) *)
     (NOTOWN: is_owned own p = false),
     step_dropplace (Dropplace f None ((p, full) :: ps) k le own m) E0
-      (Dropplace f None ((p, full) :: ps) k le own m)
+      (Dropplace f None ps k le own m)
 | step_dropplace_init2: forall f p ps k le own m st (full: bool)
     (OWN: is_owned own p = true)
-    (DPLACE: st = drop_fully_owned (if full then split_fully_own_place p (typeof_place p) else [p])),
+    (DPLACE: st = (if full then gen_drop_place_state p else drop_fully_owned_box [p])),
     step_dropplace (Dropplace f None ((p, full) :: ps) k le own m) E0
       (Dropplace f (Some st) ps k le own m)
 | step_dropplace_box: forall le m m' k ty b' ofs' f b ofs p own ps l
@@ -410,8 +426,8 @@ Inductive step_dropplace : state -> trace -> state -> Prop :=
     (* Simulate free semantics *)
     (FREE: extcall_free_sem ge [Vptr b' ofs'] m E0 Vundef m'),
     (* We are dropping p. fp is the fully owned place which is split into p::l *)
-    step_dropplace (Dropplace f (Some (drop_fully_owned (p :: l))) ps k le own m) E0
-      (Dropplace f (Some (drop_fully_owned l)) ps k le (move_place own p) m')
+    step_dropplace (Dropplace f (Some (drop_fully_owned_box (p :: l))) ps k le own m) E0
+      (Dropplace f (Some (drop_fully_owned_box l)) ps k le (move_place own p) m')
 | step_dropplace_struct: forall m k orgs co id p b ofs f le own ps l
     (* It corresponds to the call step to the drop glue of this struct *)
     (PTY: typeof_place p = Tstruct orgs id)
@@ -419,8 +435,8 @@ Inductive step_dropplace : state -> trace -> state -> Prop :=
     (COSTRUCT: co.(co_sv) = Struct)
     (PADDR: eval_place ge le m p b ofs),
     (* update the ownership environment in continuation *)
-    step_dropplace (Dropplace f (Some (drop_fully_owned (p :: l))) ps k le own m) E0
-      (Dropstate id (Vptr b ofs) None co.(co_members) (Kdropplace f (Some (drop_fully_owned l)) ps le (move_place own p) k) m)
+    step_dropplace (Dropplace f (Some (drop_fully_owned_comp p l)) ps k le own m) E0
+      (Dropstate id (Vptr b ofs) None co.(co_members) (Kdropplace f (Some (drop_fully_owned_box l)) ps le (move_place own p) k) m)
 | step_dropplace_enum: forall m k p orgs co id fid fty tag b ofs f le own ps l
     (PTY: typeof_place p = Tvariant orgs id)
     (SCO: ge.(genv_cenv) ! id = Some co)
@@ -432,10 +448,10 @@ Inductive step_dropplace : state -> trace -> state -> Prop :=
     (* use tag to choose the member *)
     (MEMB: list_nth_z co.(co_members) (Int.unsigned tag) = Some (Member_plain fid fty)),
     (* update the ownership environment in continuation *)
-    step_dropplace (Dropplace f (Some (drop_fully_owned (p :: l))) ps k le own m) E0
-      (Dropstate id (Vptr b ofs) (type_to_drop_member_state ge fid fty) nil (Kdropplace f (Some (drop_fully_owned l)) ps le (move_place own p) k) m)
+    step_dropplace (Dropplace f (Some (drop_fully_owned_comp p l)) ps k le own m) E0
+      (Dropstate id (Vptr b ofs) (type_to_drop_member_state ge fid fty) nil (Kdropplace f (Some (drop_fully_owned_box l)) ps le (move_place own p) k) m)
 | step_dropplace_next: forall f ps k le own m,
-    step_dropplace (Dropplace f (Some (drop_fully_owned nil)) ps k le own m) E0
+    step_dropplace (Dropplace f (Some (drop_fully_owned_box nil)) ps k le own m) E0
       (Dropplace f None ps k le own m)
 | step_dropplace_return: forall f k le own m,
     step_dropplace (Dropplace f None nil k le own m) E0
